Imps/Imp/Smallstep.v
@@ -1,8 +1,6 @@
 Add Rec LoadPath "~/Code/Coq".
 
-Require Import ImpSyntax.
-
-(** * Structural operational semantics for IMP *)
+Require Export Syntax.
 
 Inductive AEval (s : State) : AExp -> AExp -> Prop :=
     | AEval_Var :
@@ -37,16 +35,6 @@ match goal with
     | H1 : AEval ?s ?a ?a1, H2 : AEval ?s ?a ?a2 |- _ =>
         assert (a1 = a2) by (eapply AEval_det; eauto); subst; clear H2
 end.
-
-Inductive rtc {A : Type} (R : A -> A -> Prop) : A -> A -> Prop :=
-    | rtc_step :
-        forall x y : A, R x y -> rtc R x y
-    | rtc_refl :
-        forall x : A, rtc R x x
-    | rtc_trans :
-        forall x y z : A, rtc R x y -> rtc R y z -> rtc R x z.
-
-Hint Constructors rtc.
 
 Inductive AEvals (s : State) : AExp -> AExp -> Prop :=
     | AEvals_step :
@@ -90,45 +78,6 @@ Lemma AEvals_ABinOp :
   forall (s : State) (f : nat -> nat -> nat) (n1 n2 : nat),
     AEvals s (ABinOp f (AConst n1) (AConst n2)) (AConst (f n1 n2)).
 Proof. eauto. Qed.
-
-Lemma aeval_AEvals :
-  forall (s : State) (a : AExp) (n : nat),
-    aeval s a = n -> AEvals s a (AConst n).
-Proof.
-  induction a; cbn; intros.
-    inv H. auto.
-    inv H. eauto.
-    specialize (IHa1 _ eq_refl). specialize (IHa2 _ eq_refl).
-      eapply AEvals_trans.
-        Focus 2. rewrite <- H. apply AEvals_ABinOp.
-      eapply AEvals_trans.
-        apply AEvals_ABinOp_L. eassumption.
-      apply AEvals_ABinOp_R. assumption.
-Qed.
-
-Lemma AEval_aevals :
-  forall {s : State} {a1 a2 : AExp},
-    AEval s a1 a2 -> aeval s a1 = aeval s a2.
-Proof.
-  induction 1; cbn; auto.
-Qed.
-
-Lemma AEvals_aevals :
-  forall (s : State) (a1 a2 : AExp),
-    AEvals s a1 a2 -> aeval s a1 = aeval s a2.
-Proof.
-  induction 1; cbn; intros.
-    apply AEval_aevals. assumption.
-    reflexivity.
-    rewrite IHAEvals1. assumption.
-Qed.
-
-Lemma AEvals_aeval :
-  forall (s : State) (a : AExp) (n : nat),
-    AEvals s a (AConst n) -> aeval s a = n.
-Proof.
-  intros. apply AEvals_aevals in H. cbn in H. assumption.
-Qed.
 
 Lemma AEval_acompatible_det :
   forall {s1 : State} {a a1 : AExp},
@@ -194,15 +143,6 @@ match goal with
         assert (e1 = e2) by (eapply BEval_det; eauto); subst; clear H2
 end.
 
-Lemma BEval_bevals :
-  forall {s : State} {e1 e2 : BExp},
-    BEval s e1 e2 -> beval s e1 = beval s e2.
-Proof.
-  Hint Resolve AEval_aevals.
-  induction 1; cbn;
-  rewrite ?(AEval_aevals H), ?IHBEval, ?IHBEval1, ?IHBEval2; auto.
-Qed.
-
 Definition BEvals (s : State) (e1 e2 : BExp) : Prop :=
   rtc (BEval s) e1 e2.
 
@@ -265,45 +205,6 @@ Hint Resolve
   BEvals_Not_Step BEvals_Not
   BEvals_BBinOp_L BEvals_BBinOp_R BEvals_BBinOp.
 
-Lemma beval_BEvals :
-  forall (s : State) (e : BExp) (b : bool),
-    beval s e = b -> BEvals s e (BConst b).
-Proof.
-  Hint Unfold BEvals.
-  induction e; cbn; intros.
-    inv H. auto.
-    inv H. eapply rtc_trans.
-      apply BEvals_BRelOp_L. apply aeval_AEvals. reflexivity.
-      eapply rtc_trans.
-        apply BEvals_BRelOp_R. apply aeval_AEvals. reflexivity.
-        apply BEvals_BRelOp.
-    inv H. eapply rtc_trans.
-      apply BEvals_Not_Step. apply IHe. reflexivity.
-      apply BEvals_Not.
-    inv H. eapply rtc_trans.
-      apply BEvals_BBinOp_L. apply IHe1. reflexivity.
-      eapply rtc_trans.
-        apply BEvals_BBinOp_R. apply IHe2. reflexivity.
-        apply BEvals_BBinOp.
-Qed.
-
-Lemma BEvals_bevals :
-  forall {s : State} {e1 e2 : BExp},
-    BEvals s e1 e2 -> beval s e1 = beval s e2.
-Proof.
-  induction 1; cbn; intros.
-    apply BEval_bevals. assumption.
-    reflexivity.
-    rewrite IHrtc1, IHrtc2. reflexivity.
-Qed.
-
-Lemma BEvals_beval :
-  forall (s : State) (e : BExp) (b : bool),
-    BEvals s e (BConst b) -> beval s e = b.
-Proof.
-  intros. apply BEvals_bevals in H. cbn in H. assumption.
-Qed.
-
 Lemma BEval_bcompatible_det :
   forall {s1 : State} {e e1 : BExp},
     BEval s1 e e1 -> forall {s2 : State},
@@ -351,7 +252,7 @@ Inductive CEval : Com * State -> Com * State -> Prop :=
 
 Hint Constructors CEval.
 
-Lemma while_true_do_skip :
+Example while_true_do_skip :
   forall s1 s2 : State,
     ~ CEval (While (BConst true) Skip, s1) (Skip, s2).
 Proof.
@@ -389,36 +290,6 @@ Definition CEvals (cs1 cs2 : Com * State) : Prop :=
   rtc CEval cs1 cs2.
 
 Hint Unfold CEvals.
-
-Lemma CEval_cevals :
-  forall {cs1 cs2 : Com * State},
-    CEval cs1 cs2 -> forall (n : nat) (s : State),
-      ceval n (fst cs2) (snd cs2) = Some s ->
-      ceval (S n) (fst cs1) (snd cs1) = Some s.
-Proof.
-  induction 1; cbn; intros [| fuel] final Heq;
-  try (cbn in *; congruence; fail).
-    cbn in *. rewrite <- Heq. do 2 f_equal. apply AEval_aevals. assumption.
-    Focus 2. cbn in Heq. apply BEval_bevals in H. rewrite <- Heq, H.
-      destruct (beval s b').
-        all: rewrite Heq; change (S fuel) with (1 + fuel); rewrite plus_comm;
-          apply ceval_plus; assumption.
-    Focus 2. cbn in Heq. destruct (beval s b).
-      destruct fuel; cbn in Heq.
-        inv Heq.
-        destruct (ceval fuel c s) eqn: Heq'.
-          change (S (S fuel)) with (2 + fuel).
-            rewrite (ceval_plus' Heq' 2).
-            rewrite (ceval_plus' Heq 2). reflexivity.
-          inv Heq.
-      destruct fuel; inv Heq. reflexivity.
-    cbn in Heq. unfold fst, snd in *.
-      destruct (ceval fuel c1' s') eqn: Heq'.
-        specialize (IHCEval _ _ Heq'). rewrite IHCEval.
-          change (S fuel) with (1 + fuel). rewrite (ceval_plus' Heq 1).
-          reflexivity.
-        inv Heq.
-Qed.
 
 Lemma CEvals_Asgn_Step :
   forall (s : State) (a a' : AExp) (x : Loc),
@@ -476,6 +347,139 @@ Lemma CEvals_While :
     CEvals (While b c, s) (If b (Seq c (While b c)) Skip, s).
 Proof. eauto. Qed.
 
+Definition CEvals' (cs1 cs2 : Com * State) : Prop :=
+  rtc' CEval cs1 cs2.
+
+Hint Unfold CEvals'.
+
+Lemma CEvals_CEvals' :
+  forall cs1 cs2 : Com * State,
+    CEvals cs1 cs2 -> CEvals' cs1 cs2.
+Proof.
+  unfold CEvals; unfold CEvals'.
+  induction 1; eauto.
+  eapply rtc'_trans; eauto.
+Qed.
+
+Require Import Denotational.
+
+Lemma aeval_AEvals :
+  forall (s : State) (a : AExp) (n : nat),
+    aeval s a = n -> AEvals s a (AConst n).
+Proof.
+  induction a; cbn; intros.
+    inv H. auto.
+    inv H. eauto.
+    specialize (IHa1 _ eq_refl). specialize (IHa2 _ eq_refl).
+      eapply AEvals_trans.
+        Focus 2. rewrite <- H. apply AEvals_ABinOp.
+      eapply AEvals_trans.
+        apply AEvals_ABinOp_L. eassumption.
+      apply AEvals_ABinOp_R. assumption.
+Qed.
+
+Lemma AEval_aevals :
+  forall {s : State} {a1 a2 : AExp},
+    AEval s a1 a2 -> aeval s a1 = aeval s a2.
+Proof.
+  induction 1; cbn; auto.
+Qed.
+
+Lemma AEvals_aevals :
+  forall (s : State) (a1 a2 : AExp),
+    AEvals s a1 a2 -> aeval s a1 = aeval s a2.
+Proof.
+  induction 1; cbn; intros.
+    apply AEval_aevals. assumption.
+    reflexivity.
+    rewrite IHAEvals1. assumption.
+Qed.
+
+Lemma AEvals_aeval :
+  forall (s : State) (a : AExp) (n : nat),
+    AEvals s a (AConst n) -> aeval s a = n.
+Proof.
+  intros. apply AEvals_aevals in H. cbn in H. assumption.
+Qed.
+
+Lemma BEval_bevals :
+  forall {s : State} {e1 e2 : BExp},
+    BEval s e1 e2 -> beval s e1 = beval s e2.
+Proof.
+  Hint Resolve AEval_aevals.
+  induction 1; cbn;
+  rewrite ?(AEval_aevals H), ?IHBEval, ?IHBEval1, ?IHBEval2; auto.
+Qed.
+
+Lemma beval_BEvals :
+  forall (s : State) (e : BExp) (b : bool),
+    beval s e = b -> BEvals s e (BConst b).
+Proof.
+  Hint Unfold BEvals.
+  induction e; cbn; intros.
+    inv H. auto.
+    inv H. eapply rtc_trans.
+      apply BEvals_BRelOp_L. apply aeval_AEvals. reflexivity.
+      eapply rtc_trans.
+        apply BEvals_BRelOp_R. apply aeval_AEvals. reflexivity.
+        apply BEvals_BRelOp.
+    inv H. eapply rtc_trans.
+      apply BEvals_Not_Step. apply IHe. reflexivity.
+      apply BEvals_Not.
+    inv H. eapply rtc_trans.
+      apply BEvals_BBinOp_L. apply IHe1. reflexivity.
+      eapply rtc_trans.
+        apply BEvals_BBinOp_R. apply IHe2. reflexivity.
+        apply BEvals_BBinOp.
+Qed.
+
+Lemma BEvals_bevals :
+  forall {s : State} {e1 e2 : BExp},
+    BEvals s e1 e2 -> beval s e1 = beval s e2.
+Proof.
+  induction 1; cbn; intros.
+    apply BEval_bevals. assumption.
+    reflexivity.
+    rewrite IHrtc1, IHrtc2. reflexivity.
+Qed.
+
+Lemma BEvals_beval :
+  forall (s : State) (e : BExp) (b : bool),
+    BEvals s e (BConst b) -> beval s e = b.
+Proof.
+  intros. apply BEvals_bevals in H. cbn in H. assumption.
+Qed.
+
+Lemma CEval_cevals :
+  forall {cs1 cs2 : Com * State},
+    CEval cs1 cs2 -> forall (n : nat) (s : State),
+      ceval n (fst cs2) (snd cs2) = Some s ->
+      ceval (S n) (fst cs1) (snd cs1) = Some s.
+Proof.
+  induction 1; cbn; intros [| fuel] final Heq;
+  try (cbn in *; congruence; fail).
+    cbn in *. rewrite <- Heq. do 2 f_equal. apply AEval_aevals. assumption.
+    Focus 2. cbn in Heq. apply BEval_bevals in H. rewrite <- Heq, H.
+      destruct (beval s b').
+        all: rewrite Heq; change (S fuel) with (1 + fuel); rewrite plus_comm;
+          apply ceval_plus; assumption.
+    Focus 2. cbn in Heq. destruct (beval s b).
+      destruct fuel; cbn in Heq.
+        inv Heq.
+        destruct (ceval fuel c s) eqn: Heq'.
+          change (S (S fuel)) with (2 + fuel).
+            rewrite (ceval_plus' Heq' 2).
+            rewrite (ceval_plus' Heq 2). reflexivity.
+          inv Heq.
+      destruct fuel; inv Heq. reflexivity.
+    cbn in Heq. unfold fst, snd in *.
+      destruct (ceval fuel c1' s') eqn: Heq'.
+        specialize (IHCEval _ _ Heq'). rewrite IHCEval.
+          change (S fuel) with (1 + fuel). rewrite (ceval_plus' Heq 1).
+          reflexivity.
+        inv Heq.
+Qed.
+
 Lemma ceval_CEvals :
   forall (n : nat) (c : Com) (s s' : State),
     ceval n c s = Some s' -> CEvals (c, s) (Skip, s').
@@ -518,38 +522,6 @@ Proof.
         eapply rtc_trans.
           apply CEvals_If_False.
           inv H. auto.
-Qed.
-
-Inductive rtc' {A : Type} (R : A -> A -> Prop) : A -> A -> Prop :=
-    | rtc'_refl :
-        forall x : A, rtc' R x x
-    | rtc'_steptrans :
-        forall x y z : A, R x y -> rtc' R y z -> rtc' R x z.
-
-Hint Constructors rtc'.
-
-Definition CEvals' (cs1 cs2 : Com * State) : Prop :=
-  rtc' CEval cs1 cs2.
-
-Hint Unfold CEvals'.
-
-Lemma rtc'_trans :
-  forall {A : Type} {R : A -> A -> Prop} {x y z : A},
-    rtc' R x y -> rtc' R y z -> rtc' R x z.
-Proof.
-  intros until 1. revert z.
-  induction H; intros.
-    assumption.
-    eauto.
-Qed.
-
-Lemma CEvals_CEvals' :
-  forall cs1 cs2 : Com * State,
-    CEvals cs1 cs2 -> CEvals' cs1 cs2.
-Proof.
-  unfold CEvals; unfold CEvals'.
-  induction 1; eauto.
-  eapply rtc'_trans; eauto.
 Qed.
 
 Lemma CEvals'_ceval :
@@ -596,109 +568,3 @@ Lemma CEvals_ceval :
 Proof.
   intros. apply CEvals'_ceval, CEvals_CEvals'. assumption.
 Qed.
-
-Require Imp_BigStep.
-
-Lemma Imp_BigStep_SmallStep_AExp :
-  forall (s : State) (a : AExp) (n : nat),
-    Imp_BigStep.AEval a s n <-> AEvals s a (AConst n).
-Proof.
-  split; intro.
-    apply Imp_BigStep.AEval_aeval in H. apply aeval_AEvals. assumption.
-    apply AEvals_aeval in H. apply Imp_BigStep.aeval_AEval. assumption.
-Qed.
-Lemma Imp_BigStep_SmallStep_BExp :
-  forall (s : State) (e : BExp) (b : bool),
-    Imp_BigStep.BEval e s b <-> BEvals s e (BConst b).
-Proof.
-  split; intro.
-    apply Imp_BigStep.BEval_beval in H. apply beval_BEvals. assumption.
-    apply BEvals_beval in H. apply Imp_BigStep.beval_BEval. assumption.
-Qed.
-
-Lemma Imp_BigStep_SmallStep_Com :
-  forall (c : Com) (s1 s2 : State),
-    Imp_BigStep.CEval c s1 s2 <-> CEvals (c, s1) (Skip, s2).
-Proof.
-  split; intro.
-    apply Imp_BigStep.CEval_ceval in H. destruct H as [n H].
-      eapply ceval_CEvals. eassumption.
-    apply CEvals_ceval in H. destruct H as [n H].
-      apply Imp_BigStep.ceval_CEval with n. assumption.
-Qed.
-
-(*
-Lemma CEval_not_In_locw_eq :
-  forall (c : Com) (s1 s2 : State),
-    CEval c s1 s2 -> forall x : Loc, ~ In x (locw c) -> s1 x = s2 x.
-Proof.
-  induction 1; cbn in *; intros; auto.
-    unfold changeState. destruct (dec_spec v x).
-      subst. contradiction H0. left. reflexivity.
-      reflexivity.
-    all: rewrite ?IHCEval, ?IHCEval1, ?IHCEval2; auto.
-Qed.
-
-
-Lemma CEval_not_In_loc_eq :
-  forall (c : Com) (s1 s2 : State),
-    CEval c s1 s2 -> forall x : Loc, ~ In x (loc c) -> s1 x = s2 x.
-Proof.
-  induction 1; cbn in *; intros; auto.
-    unfold changeState. destruct (dec_spec v x).
-      subst. contradiction H0. left. reflexivity.
-      reflexivity.
-    all: rewrite ?IHCEval, ?IHCEval1, ?IHCEval2; auto 7.
-Qed.
-
-Lemma CEval_ccompatible :
-  forall (c : Com) (s1 s2 : State),
-    CEval c s1 s2 ->
-    forall {s1' s2' : State},
-      CEval c s1' s2' ->
-        ccompatible c s1 s1' -> ccompatible c s2 s2'.
-Proof.
-  unfold ccompatible.
-  Hint Unfold bcompatible.
-  induction 1; cbn; intros.
-    inv H1.
-    inv H0. unfold changeState. inv H2.
-      destruct (dec_spec x x).
-        eapply AEval_acompatible_det; eauto.
-        contradiction.
-      destruct (dec_spec v x).
-        eapply AEval_acompatible_det; eauto.
-        auto.
-    Focus 4. inv H0.
-      apply H1. assumption.
-      assert (false = true).
-        eapply BEval_bcompatible_det; eauto. congruence.
-(* If *)
-(*
-    Focus 2. inv H1.
-      eapply IHCEval; eauto 6.
-*)
-(* Seq *)
-(*
-    inv H1. apply in_app_or in H3. destruct H3.
-      assert (In x (loc c2) \/ ~ In x (loc c2)).
-        admit.
-        destruct H3.
-          assert (ccompatible c1 s2 s4).
-            red. intros. eapply IHCEval1; eauto.
-            red in H4. eapply IHCEval2; eauto. intros.
-              apply H4. assumption.
-*)
-(* While *)
-(*
-    Focus 4. inv H2; cbn in *.
-      assert (false = true); try congruence.
-        eapply BEval_bcompatible_det; eauto. unfold bcompatible.
-          intros. symmetry. auto.
-      assert (s1 x = s1' x).
-        apply H3. assumption.
-        assert (s3 x = s2' x).
-          eapply IHCEval2; eauto. intros. apply in_app_or in H5. inv H5.
-*)
-Abort.
-*)
