Imps/Imp/Syntax.v
@@ -1,4 +1,4 @@
-Add LoadPath "~/Code/Coq".
+Add Rec LoadPath "~/Code/Coq".
 
 Require Export Recdef.
 
@@ -29,13 +29,6 @@ Definition initialState : State := fun _ => 0.
 Definition changeState (s : State) (x : Loc) (n : nat) : State :=
   fun y : Loc => if x =? y then n else s y.
 
-Fixpoint aeval (s : State) (a : AExp) : nat :=
-match a with
-    | AConst n => n
-    | Var v => s v
-    | ABinOp f a1 a2 => f (aeval s a1) (aeval s a2)
-end.
-
 Fixpoint loca (a : AExp) : list Loc :=
 match a with
     | AConst _ => []
@@ -45,14 +38,6 @@ end.
 
 Definition acompatible (a : AExp) (s1 s2 : State) : Prop :=
   forall x : Loc, In x (loca a) -> s1 x = s2 x.
-
-Fixpoint beval (s : State) (e : BExp) : bool :=
-match e with
-    | BConst b => b
-    | BRelOp f a1 a2 => f (aeval s a1) (aeval s a2)
-    | Not e' => negb (beval s e')
-    | BBinOp f e1 e2 => f (beval s e1) (beval s e2)
-end.
 
 Fixpoint locb (b : BExp) : list Loc :=
 match b with
@@ -64,56 +49,6 @@ end.
 
 Definition bcompatible (b : BExp) (s1 s2 : State) : Prop :=
   forall x : Loc, In x (locb b) -> s1 x = s2 x.
-
-Function ceval (n : nat) (c : Com) (s : State) : option State :=
-match n with
-    | 0 => None
-    | S n' =>
-        match c with
-            | Skip => Some s
-            | Asgn x a => Some (changeState s x (aeval s a))
-            | Seq c1 c2 =>
-                match ceval n' c1 s with
-                    | None => None
-                    | Some s' => ceval n' c2 s'
-                end
-            | If b c1 c2 =>
-                if beval s b then ceval n' c1 s else ceval n' c2 s
-            | While b c =>
-                if beval s b
-                then
-                  match ceval n' c s with
-                      | None => None
-                      | Some s' => ceval n' (While b c) s'
-                  end
-                else Some s
-        end
-end.
-
-Lemma ceval_plus :
-  forall (n k : nat) (c : Com) (s1 s2 : State),
-    ceval n c s1 = Some s2 -> ceval (n + k) c s1 = Some s2.
-Proof.
-  induction n as [| n']; cbn; intros.
-    inv H.
-    destruct c; auto.
-      destruct (ceval n' c1 s1) eqn: Heq.
-        erewrite IHn'; eauto.
-        inv H.
-      destruct (beval s1 b) eqn: Hb; eauto.
-      destruct (beval s1 b) eqn: Hb; eauto.
-        destruct (ceval n' c s1) eqn: Heq.
-          erewrite IHn'; eauto.
-          inv H.
-Qed.
-
-Lemma ceval_plus' :
-  forall {n : nat} {c : Com} {s1 s2 : State},
-    ceval n c s1 = Some s2 ->
-      forall k : nat, ceval (k + n) c s1 = Some s2.
-Proof.
-  intros. rewrite plus_comm. apply ceval_plus. assumption.
-Qed.
 
 (* The list of all variables which are assigned to by the instruction c. *)
 Fixpoint locw (c : Com) : list Loc :=
