Imps/Imp/Denotational.v
@@ -1,0 +1,68 @@
+Add Rec LoadPath "~/Code/Coq".
+
+Require Export Syntax.
+
+Fixpoint aeval (s : State) (a : AExp) : nat :=
+match a with
+    | AConst n => n
+    | Var v => s v
+    | ABinOp f a1 a2 => f (aeval s a1) (aeval s a2)
+end.
+
+Fixpoint beval (s : State) (e : BExp) : bool :=
+match e with
+    | BConst b => b
+    | BRelOp f a1 a2 => f (aeval s a1) (aeval s a2)
+    | Not e' => negb (beval s e')
+    | BBinOp f e1 e2 => f (beval s e1) (beval s e2)
+end.
+
+Function ceval (n : nat) (c : Com) (s : State) : option State :=
+match n with
+    | 0 => None
+    | S n' =>
+        match c with
+            | Skip => Some s
+            | Asgn x a => Some (changeState s x (aeval s a))
+            | Seq c1 c2 =>
+                match ceval n' c1 s with
+                    | None => None
+                    | Some s' => ceval n' c2 s'
+                end
+            | If b c1 c2 =>
+                if beval s b then ceval n' c1 s else ceval n' c2 s
+            | While b c =>
+                if beval s b
+                then
+                  match ceval n' c s with
+                      | None => None
+                      | Some s' => ceval n' (While b c) s'
+                  end
+                else Some s
+        end
+end.
+
+Lemma ceval_plus :
+  forall (n k : nat) (c : Com) (s1 s2 : State),
+    ceval n c s1 = Some s2 -> ceval (n + k) c s1 = Some s2.
+Proof.
+  induction n as [| n']; cbn; intros.
+    inv H.
+    destruct c; auto.
+      destruct (ceval n' c1 s1) eqn: Heq.
+        erewrite IHn'; eauto.
+        inv H.
+      destruct (beval s1 b) eqn: Hb; eauto.
+      destruct (beval s1 b) eqn: Hb; eauto.
+        destruct (ceval n' c s1) eqn: Heq.
+          erewrite IHn'; eauto.
+          inv H.
+Qed.
+
+Lemma ceval_plus' :
+  forall {n : nat} {c : Com} {s1 s2 : State},
+    ceval n c s1 = Some s2 ->
+      forall k : nat, ceval (k + n) c s1 = Some s2.
+Proof.
+  intros. rewrite plus_comm. apply ceval_plus. assumption.
+Qed.
