Imps/Imp/SmallstepBigstep.v
@@ -1,0 +1,35 @@
+Add Rec LoadPath "~/Code/Coq".
+
+Require Export Syntax.
+
+Require Imp.Smallstep.
+Require Imp.Bigstep.
+
+Lemma Bigstep_Smallstep_AExp :
+  forall (s : State) (a : AExp) (n : nat),
+    Bigstep.AEval a s n <-> Smallstep.AEvals s a (AConst n).
+Proof.
+  split; intro.
+    apply Bigstep.AEval_aeval in H. apply Smallstep.aeval_AEvals. assumption.
+    apply Smallstep.AEvals_aeval in H. apply Bigstep.aeval_AEval. assumption.
+Qed.
+
+Lemma Bigstep_Smallstep_BExp :
+  forall (s : State) (e : BExp) (b : bool),
+    Bigstep.BEval e s b <-> Smallstep.BEvals s e (BConst b).
+Proof.
+  split; intro.
+    apply Bigstep.BEval_beval in H. apply Smallstep.beval_BEvals. assumption.
+    apply Smallstep.BEvals_beval in H. apply Bigstep.beval_BEval. assumption.
+Qed.
+
+Lemma Bigstep_Smallstep_Com :
+  forall (c : Com) (s1 s2 : State),
+    Bigstep.CEval c s1 s2 <-> Smallstep.CEvals (c, s1) (Skip, s2).
+Proof.
+  split; intro.
+    apply Bigstep.CEval_ceval in H. destruct H as [n H].
+      eapply Smallstep.ceval_CEvals. eassumption.
+    apply Smallstep.CEvals_ceval in H. destruct H as [n H].
+      apply Bigstep.ceval_CEval with n. assumption.
+Qed.
