Imps/Imp/SmallstepWithContexts.v
@@ -1,0 +1,188 @@
+Add Rec LoadPath "~/Code/Coq".
+
+Require Import Syntax.
+
+(** * Structural operational semantics for IMP using contexts *)
+
+Inductive AStep (s : State) : AExp -> AExp -> Prop :=
+    | AStep_Var :
+        forall x : Loc, AStep s (Var x) (AConst (s x))
+    | AStep_ABinOp :
+        forall (f : nat -> nat -> nat) (n1 n2 : nat),
+          AStep s (ABinOp f (AConst n1) (AConst n2)) (AConst (f n1 n2)).
+
+Inductive AContext : Type :=
+    | AC_Var : AContext
+    | AC_L : (nat -> nat -> nat) -> AContext -> AExp -> AContext
+    | AC_R : (nat -> nat -> nat) -> nat -> AContext -> AContext.
+
+Fixpoint aput (G : AContext) (a : AExp) : AExp :=
+match G with
+    | AC_Var => a
+    | AC_L f G' a' => ABinOp f (aput G' a) a'
+    | AC_R f n G' => ABinOp f (AConst n) (aput G' a)
+end.
+
+Inductive AEval (s : State) : AExp -> AExp -> Prop :=
+    | AEval_aput :
+        forall (a1 a2 : AExp) (G : AContext),
+          AStep s a1 a2 -> AEval s (aput G a1) (aput G a2).
+
+Hint Constructors AStep AEval.
+
+Require Import Recdef.
+
+(*
+Function AExp_to_AContext (a : AExp) : AContext * AExp :=
+match a with
+    | AConst n => (AC_Var, AConst n)
+    | Var x => (AC_Var, Var x)
+    | ABinOp f (AConst n) a2 =>
+        let '(G, a) := AExp_to_AContext a2 in (AC_R f n G, a)
+    | ABinOp f a1 a2 =>
+        let '(G, a) := AExp_to_AContext a1 in (AC_L f G a2, a)
+end.
+
+Lemma AExp_to_AContext_aput :
+  forall (a1 a2 : AExp) (G : AContext),
+    AExp_to_AContext a1 = (G, a2) -> aput G a2 = a1.
+Proof.
+  intros a1.
+  functional induction AExp_to_AContext a1;
+    intros; inv H; cbn; f_equal; auto.
+Qed.
+
+Lemma AExp_to_AContext_aput' :
+  forall a : AExp,
+    aput (fst (AExp_to_AContext a)) (snd (AExp_to_AContext a)) = a.
+Proof.
+  intros. apply AExp_to_AContext_aput.
+  destruct AExp_to_AContext. cbn. reflexivity.
+Qed.
+*)
+
+Require Imp.Smallstep.
+
+Lemma AEval_Smallstep_AEval :
+  forall (s : State) (a1 a2 : AExp),
+    AEval s a1 a2 <-> Smallstep.AEval s a1 a2.
+Proof.
+  split.
+    intro. inv H. induction G; cbn; auto. induction H0; auto.
+    induction 1.
+      change (Var x)
+        with (aput AC_Var (Var x));
+      change (AConst (s x))
+        with (aput AC_Var (AConst (s x))).
+        constructor. constructor.
+      inv IHAEval.
+        change (ABinOp f (aput G a0) a2)
+          with (aput (AC_L f G a2) a0).
+        change (ABinOp f (aput G a3) a2)
+          with (aput (AC_L f G a2) a3).
+        constructor. assumption.
+      inv IHAEval.
+        change (ABinOp f (AConst n) (aput G a1))
+          with (aput (AC_R f n G) a1).
+        change (ABinOp f (AConst n) (aput G a0))
+          with (aput (AC_R f n G) a0).
+        constructor. assumption.
+      change (ABinOp f (AConst n1) (AConst n2))
+        with (aput AC_Var (ABinOp f (AConst n1) (AConst n2)));
+      change (AConst (f n1 n2))
+        with (aput AC_Var (AConst (f n1 n2))).
+        constructor. constructor.
+Qed.
+
+Inductive BStep : BExp -> BExp -> Prop :=
+    | BStep_BRelOp :
+        forall (f : nat -> nat -> bool) (n1 n2 : nat),
+          BStep (BRelOp f (AConst n1) (AConst n2)) (BConst (f n1 n2))
+    | BStep_Not :
+        forall b : bool, BStep (Not (BConst b)) (BConst (negb b))
+    | BStep_BBinOp :
+        forall (f : bool -> bool -> bool) (b1 b2 : bool),
+          BStep (BBinOp f (BConst b1) (BConst b2)) (BConst (f b1 b2)).
+
+Print BExp.
+
+Inductive BContext : Type :=
+    | BC_Hole : BContext
+(*
+    | BC_BRelOp_L : (nat -> nat -> bool) -> BContext -> AExp -> BContext
+    | BC_BRelOp_R : (nat -> nat -> bool) -> nat -> BContext -> BContext
+*)
+    | BC_Not : BContext -> BContext
+    | BC_BBinOp_L : (bool -> bool -> bool) -> BContext -> BExp -> BContext
+    | BC_BBinOp_R : (bool -> bool -> bool) -> bool -> BContext -> BContext.
+
+Fixpoint bput (G : BContext) (e : BExp) : BExp :=
+match G with
+    | BC_Hole => e
+(*
+    | BC_BRelOp_L f G' a => BRelOp f (bput G' e) a
+    | BC_BRelOp_R f n G' => BRelOp f (AConst n) (bput G' e)
+*)
+    | BC_Not G' => Not (bput G' e)
+    | BC_BBinOp_L f G' e' => BBinOp f (bput G' e) e'
+    | BC_BBinOp_R f b G' => BBinOp f (BConst b) (bput G' e)
+end.
+
+Inductive BEval : BExp -> BExp -> Prop :=
+    | BEval_bput :
+        forall (G : BContext) (b1 b2 : BExp),
+          BStep b1 b2 -> BEval (bput G b1) (bput G b2).
+
+Lemma BEval_Smallstep_BEval :
+  forall (s : State) (b1 b2 : BExp),
+    BEval b1 b2 <-> Smallstep.BEval s b1 b2.
+Proof.
+  split.
+    intro. inv H. induction G; cbn; auto. inv H0; auto.
+    induction 1.
+      admit.
+      admit.
+      {
+        change (BRelOp f (AConst n1) (AConst n2))
+          with (bput BC_Hole (BRelOp f (AConst n1) (AConst n2))).
+        change (BConst (f n1 n2 ))
+          with (bput BC_Hole (BConst (f n1 n2))).
+        constructor. constructor.
+      }
+      {
+        inv IHBEval.
+        change (Not (bput G b1)) with (bput (BC_Not G) b1).
+        change (Not (bput G b2)) with (bput (BC_Not G) b2).
+        constructor. assumption.
+      }
+      {
+        change (Not (BConst b))
+          with (bput BC_Hole (Not (BConst b))).
+        change (BConst (negb b))
+          with (bput BC_Hole (BConst (negb b))).
+        constructor. constructor.
+      }
+      {
+        inv IHBEval.
+        change (BBinOp f (bput G b1) e2)
+          with (bput (BC_BBinOp_L f G e2) b1).
+        change (BBinOp f (bput G b2) e2)
+          with (bput (BC_BBinOp_L f G e2) b2).
+        constructor. assumption.
+      }
+      {
+        inv IHBEval.
+        change (BBinOp f (BConst b) (bput G b1))
+          with (bput (BC_BBinOp_R f b G) b1).
+        change (BBinOp f (BConst b) (bput G b2))
+          with (bput (BC_BBinOp_R f b G) b2).
+        constructor. assumption.
+      }
+      {
+        change (BBinOp f (BConst b1) (BConst b2))
+          with (bput BC_Hole (BBinOp f (BConst b1) (BConst b2))).
+        change (BConst (f b1 b2))
+          with (bput BC_Hole (BConst (f b1 b2))).
+        constructor. constructor.
+      }
+Admitted.
